C denot_set

DenotationalLean/Denot.lean
@@ -6,9 +6,11 @@ import Mathlib.Data.Part
 
 open Classical
 
+@[simp, grind]
 def a_denot : Aexp -> State -> Nat :=
   fun a => fun σ => a_eval a σ
 
+@[simp, grind]
 def b_denot : Bexp -> State -> Bool :=
   fun b => fun σ => b_eval b σ
 
@@ -28,8 +30,9 @@ theorem c_denot_correct :
   . intro h
     have ex : ∃ σ', ⟨c,σ⟩ ~~> σ' := ⟨σ', h⟩
     have _ := choose_spec ex
-    grind [c_unique]
+    grind
 
+@[simp, grind]
 def a_denot_set (a : Aexp) : Set (State × Nat) :=
   match a with
   | .Nat n => {(σ,n) | σ : State}
@@ -44,17 +47,18 @@ theorem a_denot_equiv :
   intro a σ
   induction a with
   | Nat | Loc =>
-    simp [a_denot_set, a_denot, a_eval]
+    simp
   | Add a0 a1 | Sub a0 a1 | Mul a0 a1 =>
-    simp [a_denot_set, a_denot, a_eval]
+    simp
     intro n
     apply Iff.intro
     . intro h
       use a_denot a0 σ
       use a_denot a1 σ
-      grind [a_denot]
-    . grind [a_denot]
+      grind
+    . grind
 
+@[simp, grind]
 def b_denot_set (b : Bexp) : Set (State × Bool) :=
   match b with
   | .Bool t => {(σ,t) | σ : State}
@@ -68,4 +72,57 @@ theorem b_denot_equiv :
   ∀ (b : Bexp) (σ : State) (t : Bool) , b_denot b σ = t <-> (σ,t) ∈ b_denot_set b
 := by
   intro b
-  induction b <;> simp [b_denot_set, b_denot, b_eval] <;> grind [b_denot]
+  induction b <;> simp <;> grind
+
+def fix (Γ : Set α -> Set α) : Set α := ⋃ n:Nat , n.iterate Γ ∅
+
+@[simp, grind]
+def c_denot_set (c : Com) : Set (State × State) :=
+  match c with
+  | .Skp => {(σ,σ) | σ : State}
+  | .Assign l a => {(σ,(l,a_eval a σ)::σ) | σ : State}
+  | .Seq c0 c1 => {(σ,σ') | ∃ (σ'' : State) , (σ,σ'') ∈ c_denot_set c0 ∧ (σ'',σ') ∈ c_denot_set c1}
+  | .Ite b c0 c1 => {(σ,σ') | (b_eval b σ = true) ∧ (σ,σ') ∈ c_denot_set c0} ∪ {(σ,σ') | (b_eval b σ = false) ∧ (σ,σ') ∈ c_denot_set c1}
+  | .Wh b c => fix (fun φ => {(σ,σ') | (b_eval b σ = true) ∧ ∃ (σ'' : State) , (σ,σ'') ∈ c_denot_set c ∧ (σ'',σ') ∈ φ} ∪ {(σ,σ') | (b_eval b σ = false) ∧ σ' = σ})
+
+def fix_wh (b : Bexp) (c : Com) : Set (State × State) -> Set (State × State) :=
+  fun φ => {(σ,σ') | (b_eval b σ = true) ∧ ∃ (σ'' : State) , (σ,σ'') ∈ c_denot_set c ∧ (σ'',σ') ∈ φ} ∪ {(σ,σ') | (b_eval b σ = false) ∧ σ' = σ}
+
+theorem c_denot_equiv :
+  ∀ (c : Com) (σ σ' : State) , ⟨c,σ⟩ ~~> σ' <-> (σ,σ') ∈ c_denot_set c
+:= by
+  intro c σ σ'
+  apply Iff.intro
+  . intro h
+    induction h with
+    | skip | assign | seq | ite_true | ite_false => simp [c_denot_set] <;> grind
+    | while_false =>
+      simp [c_denot_set, fix]
+      use 1
+      simp ; grind
+    | while_true hb hc whc h1 h2 =>
+      simp [c_denot_set, fix] at h2
+      let ⟨n,_⟩ := h2
+      simp [c_denot_set, fix]
+      use n + 1
+      rw [Function.iterate_succ']
+      grind
+  . revert σ σ'
+    induction c with
+    | Skp | Assign | Seq | Ite => grind
+    | Wh b c ih =>
+      have aux : ∀ (n : Nat) (σ σ' : State) ,
+          (σ,σ') ∈ (fix_wh b c)^[n] ∅ -> ⟨While b Do c,σ⟩ ~~> σ' := by
+        intro n
+        induction n with
+        | zero => simp [Nat.iterate]
+        | succ m ihh =>
+          intro σ σ' h
+          rw [Function.iterate_succ'] at h
+          simp [fix_wh] at h
+          cases h <;> grind
+      intro σ σ' hh
+      simp [c_denot_set, fix] at hh
+      let ⟨n,_⟩ := hh
+      apply aux n σ σ'
+      grind
